feat: sponge squeeze verification

lean/Shars/Verification/Simple/SpongeSqueeze.lean
@@ -18,6 +18,8 @@ set_option maxHeartbeats 100000
 attribute [-simp] List.getElem!_eq_getElem?_getD
 attribute [ext (iff:=false)] List.ext_getElem!
 
+open Aeneas
+
 -- attribute [scalar_tac_simps] Nat.pos_of_neZero
 
 @[scalar_tac inst]
@@ -71,6 +73,18 @@ def ListIR.sponge.squeeze(d: Nat)(r: Nat)[NeZero r](dst s: List Bool): List Bool
 termination_by d - dst.length
 decreasing_by scalar_decr_tac
 
+@[simp]
+theorem ListIR.sponge.length_squeeze(d: Nat)(r: Nat)[NeZero r](dst s: List Bool)
+: (squeeze d r dst s).length = d
+:= by
+  unfold squeeze
+  split
+  case isTrue h => simp [h]
+  case isFalse h =>
+    rw [ListIR.sponge.length_squeeze]
+termination_by d - dst.length
+decreasing_by scalar_decr_tac
+
 
 theorem List.getElem!_replace_slice[Inhabited α](ls ls2: List α)(s e: Nat)
 : s ≤ e -- Proper range
@@ -100,7 +114,7 @@ theorem simple.sponge_squeeze.panic_free.spec(r: Nat)
   (dst s: List Bool)(offset : Nat)
 : s.length = 1600
 → offset < dst.length
-→ have: NeZero r := {out := Nat.not_eq_zero_of_lt r_bnd.left}
+→ have : NeZero r := {out := Nat.not_eq_zero_of_lt r_bnd.left}
   panic_free r dst s offset = ListIR.sponge.squeeze dst.length r (dst.take offset) s
 := by
   intro len_s offset_idx
@@ -130,225 +144,371 @@ theorem simple.sponge_squeeze.panic_free.spec(r: Nat)
 termination_by dst.length - offset
 decreasing_by scalar_decr_tac
 
-
-
-
-
-
-
-
-
-
-
-
-
-
-
-
-
-
-
-
-
-
-
-
-
-
-
-abbrev List.is_chunks_of(chunks: List (List α))(n: Nat) := ∀ c ∈ chunks, c.length = n
-
-@[simp_lists_simps]
-theorem List.length_flatten_of_is_chunks(n: Nat)(chunks: List (List α))
-: chunks.is_chunks_of n
-→ chunks.flatten.length = chunks.length * n
+theorem simple.sponge_squeeze.panic_free.extracted_2 (r i : Std.Usize) (dst : Std.Slice Bool)
+  (s : Std.Array Bool 1600#usize) (r_bnd : 0 < (↑r : ℕ) ∧ (↑r : ℕ) < 1600) (i_idx : (↑i : ℕ) < dst.length)
+  (no_overflow : dst.length + (↑r : ℕ) < Std.Usize.max) (i1 : Std.Usize) (__1 : [> let i1 ← i + r <])
+  (i1_post : (↑i1 : ℕ) = (↑i : ℕ) + (↑r : ℕ)) (h : i1 < dst.len) (s4 : Std.Array Bool 1600#usize)[NeZero r.val]
+  (_ : [> let s4 ← keccak_p s <])
+:
+  ∃ output,
+    sponge_squeeze_loop r
+          (if h : (↑i : ℕ) + ((↑r : ℕ) + ((↑dst : List Bool).length - ((↑i : ℕ) + (↑r : ℕ)))) ≤ Std.Usize.max then
+            ⟨List.take (↑i : ℕ) (↑dst : List Bool) ++
+                (List.take (↑r : ℕ) (↑s : List Bool) ++ List.drop ((↑i : ℕ) + (↑r : ℕ)) (↑dst : List Bool)),
+              by simp; scalar_tac⟩
+          else dst)
+          s4 i1 =
+        Std.Result.ok output ∧
+      (↑output : List Bool) = panic_free (↑r : ℕ) (↑dst : List Bool) (↑s : List Bool) (↑i : ℕ)
 := by
-  intro is_chunks
-
-  induction chunks
-  case nil => simp
-  case cons hd tl ih =>
-    simp [List.is_chunks_of] at *
-    obtain ⟨len_hd, len_flatten_tl⟩ := is_chunks
-    rw [ih (is_chunks := len_flatten_tl)]
-    simp_arith [*, Nat.add_mul]
-
-@[simp_lists_simps]
-theorem List.getElem!_cons_div_of_gt[Inhabited α](i n: Nat)(hd: α)(tl: List α)
-: n > 0 → i ≥ n → (hd :: tl)[i / n]! = tl[(i - n) / n]!
-:= by
-  intro n_pos h
-  have: i = (i - n) + n := by exact (Nat.sub_eq_iff_eq_add h).mp rfl
-  conv => lhs; rw [this, Nat.add_div_right (H := n_pos)]
-  simp
-
-@[simp_lists_simps]
-theorem List.getElem!_cons_div_of_lt[Inhabited α](i n: Nat)(hd: α)(tl: List α)
-: i < n → (hd :: tl)[i / n]! = hd
-:= by intro h; simp [Nat.div_eq_of_lt, h]
-
-@[simp_lists_simps]
-theorem List.getElem!_flatten_of_is_chunks(n: Nat)[Inhabited α](chunks: List (List α))
-: chunks.is_chunks_of n
-→ ∀ i, chunks.flatten[i]! = (chunks[i/n]!)[i%n]!
-:= by
-  intro is_chunks
-
-  assume n_pos: n > 0
-  case otherwise =>
-    simp at n_pos
-    intro i
-    rw [getElem!_default, getElem!_default]
-    · if inside: i / n < chunks.length then
-        rw [getElem!_pos]
-        case h => assumption
-        have := is_chunks (chunks[i / n]) (by simp)
-        simp [*]
-      else
-        rw [getElem!_neg]
-        case h => assumption
-        simp [default]
-    · rw [List.length_flatten_of_is_chunks (n:=n)]
-      · simp [*]
-      · assumption
-
-  induction chunks
-  case nil => simp [default]
-  case cons hd tl ih =>
-    intro i
-    simp [List.is_chunks_of] at *
-    obtain ⟨len_hd, len_flatten_tl⟩ := is_chunks
-    replace ih := ih len_flatten_tl
-    by_cases i < n
-    case pos i_hd =>
-      simp_lists
-      simp [Nat.div_eq_of_lt, Nat.mod_eq_of_lt,i_hd]
-    case neg i_tl =>
-      simp at i_tl
-      simp_lists
-      rw [ih]
-      simp [len_hd, Nat.mod_eq_sub_mod, i_tl]
-
-@[simp_lists_simps]
-private theorem List.getElem!_iterate[Inhabited α](f: α → α)(a: α)(n i: Nat)
-: (List.iterate f a n)[i]! = if i < n then f^[i] a else default
-:= by
-  split
-  case isTrue i_idx  => simp [getElem!_pos, i_idx]
-  case isFalse i_oob => simp [getElem!_neg, i_oob]
-
--- def List.sumWhileNotGt(ls: List Nat)(top: Nat) := Id.run do
---   let mut sum := 0
---   for x in ls do
---     if sum + x > top then
---       break
---     sum := sum + x
---   return sum
-
--- theorem List.getElem_flatten[Inhabited α](ls: List (List α))(i: Nat)
--- : let n := ls.map (·.length) |>.sumWhileNotGt i
---   ls.flatten[i]! = (ls[n]!)[i - n]!
--- := by sorry
-
-def ref.squeeze(s: List Bool)(n: Nat)(k: Nat := 1600)[NeZero k] :=
-  (List.iterate list_keccak_p (s.setWidth k) n).flatten
-
-attribute [-simp] List.mem_iterate in
-@[simp, simp_lists_simps]
-theorem iterate_list_keccak_p_is_chunks_of_1600(s: List Bool)(n: Nat)
-: (List.iterate ref.list_keccak_p (s.setWidth 1600) n).is_chunks_of 1600
-:= by
-  induction n generalizing s
-  case zero => simp [List.is_chunks_of]
-  case succ d' ih =>
-    unfold List.is_chunks_of at *
-    simp
-    intros chunk chunk_prev
-    rw [ih (s := ref.list_keccak_p (s.setWidth 1600))]
-    simp [*]
-
--- private theorem length_squeeze(n: Nat)(s: List Bool)
--- : (ref.squeeze s n 1600).length = n*1600
--- := by
---   unfold ref.squeeze
---   rw [List.length_flatten_of_is_chunks 1600]
---   case a => apply iterate_list_keccak_p_is_chunks_of_1600
---   simp [ref.squeeze]
-
--- private theorem getElem!_squeeze(n: Nat)(s: List Bool)
--- : (ref.squeeze s n 1600)[i]! = (ref.list_keccak_p^[i / 1600] s.setWidth)[i % 1600]!
--- := by
---   simp [ref.squeeze]
---   ref [List.getElem!_flatten_of_is_chunks]
---   sorry
-
-attribute [-simp] List.length_flatten in
-attribute [simp] length_iterate_keccak_p in
-set_option maxHeartbeats 100000000 in
-theorem simple.sponge_squeze_loop.spec (r i: Std.Usize)(input: Std.Slice Bool)(s: Aeneas.Std.Array Bool 1600#usize)
-: r.val < 1600
-→ i < input.length
-→ i.val % r.val = 0
-→ input.length + r.val < Std.Usize.max
-→ ∃ output,
-  sponge_squeeze_loop r input s i = .ok output ∧
-  output.length = input.length ∧
-  output.val = input.val.take i.val ++ ref.squeeze s.val ((input.length - i.val) / r)
-  /- output.val[j]! = input. -/
-  /- (∀ j < output.length, output.val[j]! = -/
-  /-   if i.val ≤ j then -/
-  /-     (ref.list_keccak_p s.val)[j]! -/
-  /-   else -/
-  /-     input.val[j]! -/
-:= by
-  intros r_lt i_idx i_mod_r no_overflow
-  unfold sponge_squeeze_loop
-  let* ⟨ s1, s1_def ⟩ ← Std.Array.to_slice.progress_spec
-  let* ⟨ nb_added, curr, nb_added_val, curr_len, curr_pt_val ⟩ ← add_to_vec.spec
-  · simp [*, Std.Array.to_slice]
-  let* ⟨ i1, i1_post ⟩ ← Std.Usize.add_spec
-  have: input.length ≤ (input.length / r) * 1600 := by sorry
-  split
-  case isTrue last_loop =>
-    simp [*]
-    ext j
-    · have this2: input.length - i ≤ input.length := by exact Nat.sub_le input.length i.val
-      simp [*, le_of_lt, _root_.trans this2 this]
-    assume j_idx: j < curr.length
-    case otherwise => simp_lists
-    rw [curr_pt_val]
-    case a => simpa [*] using j_idx
-    simp_lists
-    split
-    case isTrue cond =>
-      simp_ifs
-      rw [List.getElem!_flatten_of_is_chunks 1600]
-      case a => apply iterate_list_keccak_p_is_chunks_of_1600
-      simp_lists
-      have: j < (input.length / r) * 1600 := by
-        scalar_tac
-      sorry
-    rw [List.getElem!_flatten_of_is_chunks]
-    sorry
-  case isFalse has_more_loops =>
-    let* ⟨ s2, s2_post ⟩ ← keccak_p.spec'
-    let* ⟨ res, res_post_1, res_post_2 ⟩ ← spec
-
-    simp [*]
-
-theorem simple.sponge_squeze.spec (r: Std.Usize)(input: Std.Slice Bool)
-: ∃ output,
-  sponge_squeeze_loop r input s i = .ok output ∧
-  output.length = input.length ∧
-  output.val = (List.iterate ref.list_keccak_p s.val (input.length / r)).flatten.take (input.length - i.val)
-:= by
+  -- conv => rhs; ext output; enter [1,1, 2]; tactic => simp_ifs
+  simp_ifs
+  simp only [‹i.val + (r.val + (dst.length - (i.val + r.val))) ≤ Std.Usize.max›', ↓reduceDIte]
   sorry
 
--- @[progress]
-theorem simple.sponge.spec (r : Std.Usize) (bs output suffix: Std.Slice Bool)
-[NeZero r.val]
-/- (r_ne_zero: r.val ≠ 0) -/
-: ∃ output,
-  simple.sponge r bs output suffix = .ok output ∧
-  output.val = (Spec.sponge (f := Spec.Keccak.P 6 (nᵣ := 24)) (pad := Spec.«pad10*1») r.val (Array.mk <| bs.val ++ suffix.val ) output.length).toArray.toList
-:= by sorry
+set_option trace.SimpIfs true
+set_option maxRecDepth 1000000000 in
+set_option maxHeartbeats 1000000000 in
+theorem simple.sponge_squeeze.panic_free.extracted_3 (r i : Std.Usize) (dst : Std.Slice Bool)
+  (i1 : Std.Usize) (i1_post : (↑i1 : ℕ) = (↑i : ℕ) + (↑r : ℕ)) (h : i1 < dst.len)
+: (if h : i.val + r.val + dst.length - (i.val + r.val) ≤ Std.Usize.max then True else False)
+:= by
+  simp_ifs -- Does nothing.
+  have: i.val + r.val + dst.length - (i.val + r.val) ≤ Std.Usize.max := by scalar_tac
+  simp only [this, reduceDIte]
+
+
+#check Std.Usize.sub_spec'
+
+@[simp]
+theorem Aeneas.Std.Slice.val_drop{T: Type}(s: Slice T)(k: Usize)
+: (s.drop k).val = s.val.drop k.val
+:= by simp [Slice.drop]
+
+set_option maxHeartbeats 1000000 in
+set_option maxRecDepth 1000000 in
+-- set_option trace.meta.Tactic.simp true in
+set_option diagnostics true in
+theorem simple.sponge_squeeze.panic_free.refinement(r i: Std.Usize)
+  (dst: Std.Slice Bool)(s: Aeneas.Std.Array Bool 1600#usize)
+: (r_bnd: 0 < r.val ∧ r.val < 1600)
+→ i < dst.length
+→ dst.length + r.val < Std.Usize.max
+→ let _: NeZero r.val := {out:= Nat.not_eq_zero_of_lt r_bnd.left}
+  ∃ output,
+  sponge_squeeze_loop r dst s i = .ok output ∧
+  output.val = panic_free r.val dst.val s.val i.val
+:= by
+  intro r_bnd i_idx no_overflow
+  unfold simple.sponge_squeeze_loop panic_free
+  let* ⟨ i1, i1_post ⟩ ← Std.Usize.add_spec
+  split
+  . simp [Std.core.slice.index.Slice.index_mut, Std.core.slice.index.SliceIndexRangeUsizeSlice.index_mut]
+    simp_ifs
+    simp [Std.core.array.Array.index, Std.core.ops.index.IndexSliceInst, Std.core.slice.index.Slice.index, Std.core.slice.index.SliceIndexRangeUsizeSlice.index, Std.Array.to_slice]
+    simp_ifs
+    simp [Std.core.slice.Slice.copy_from_slice, List.slice, Std.Slice.len]
+    simp_ifs
+    simp
+    let* ⟨ s4, s4_post ⟩ ← keccak_p.spec'
+    simp [List.replace_slice, *, le_of_lt]
+    try simp_ifs -- TODO: Why does this not work?
+    split
+    case isFalse =>
+      scalar_tac -- contradiction
+      done
+    case isTrue h =>
+      let* ⟨ rest, rest_post⟩ ← refinement
+      simp [*]
+      done
+  . let* ⟨ nb_left, nb_left_post ⟩ ← Aeneas.Std.Usize.sub_spec'
+    simp at nb_left_post
+    simp [Std.core.slice.index.Slice.index_mut, Std.core.slice.index.SliceIndexRangeFromUsizeSlice.index_mut]
+    simp_ifs
+    simp [Std.core.array.Array.index, Std.core.ops.index.IndexSliceInst, Std.core.slice.index.Slice.index, Std.core.slice.index.SliceIndexRangeUsizeSlice.index, Std.Array.to_slice]
+    simp_ifs
+    simp [Std.core.slice.Slice.copy_from_slice, List.slice, Std.Slice.len, *, Nat.min_def, List.length_drop]
+    simp_ifs
+    simp [*]
+    try simp_ifs -- TODO: Again, why does this not work?
+    have : (dst.length - ↑i) ⊓ 1600 + i.val ≤ Std.Usize.max := by scalar_tac
+    simp [this, List.replace_slice]
+    rw [←Nat.add_sub_assoc (le_of_lt i_idx), Nat.add_comm i.val, Nat.add_sub_cancel]
+    done
+termination_by dst.length - i
+decreasing_by scalar_decr_tac
+
+theorem BitVec.toList_inj{bv bv2: BitVec n}
+: bv.toList = bv2.toList → bv = bv2
+:= by
+  intro cond
+  ext i i_idx
+  replace cond := List.getElem_of_eq cond (by simp; exact i_idx)
+  simpa [getElem_eq_getElem!] using cond
+
+
+set_option trace.SimpIfs true in
+theorem ListIR.sponge.squeeze.extracted_1 {m d : ℕ} (Z : BitVec m) (base_case : d ≤ m) (i : ℕ) (h : i < d)
+: Z.getLsbD i = if h : i < m then Z[i] else false
+:= by
+  simp_ifs at h
+
+  sorry
+
+theorem BitVec.getLsbD_eq_getElem! {x : BitVec w} {i : Nat} :
+    x.getLsbD i = x[i]! := by
+  if h: i < w then
+    simp only [getElem!_pos, h]
+    rfl
+  else
+    rw [getElem!_neg]
+    case h => assumption
+    simp [default, BitVec.getLsbD, Nat.testBit]
+    have: x.toNat >>> i = 0 := by
+      apply Nat.shiftRight_eq_zero
+      calc
+        _ < 2^w := by exact x.toFin.isLt
+        _ ≤ 2^i := by
+          apply Nat.pow_le_pow_of_le Nat.one_lt_two
+          simpa using h
+    rw [this]
+
+attribute [local simp] BitVec.getLsbD_eq_getElem! in
+theorem BitVec.toList_setWidth(bv: BitVec n)(m: Nat)
+: (bv.setWidth m).toList = bv.toList.setWidth m
+:= by
+  ext i
+  · simp
+  simp
+  assume i < m
+  case otherwise h => simp [getElem!_neg, h]
+  simp [getElem!_pos, *]
+
+set_option maxRecDepth 1000000 in
+def ListIR.sponge.squeeze.refinement(r: Nat) [NeZero r]
+    (Z: BitVec m)
+    (S: BitVec (Spec.b 6))
+: Spec.sponge.squeeze (d := d) (f := Spec.Keccak.P 6 24) r Z S =
+  (squeeze d r Z.toList S.toList).toBitVec.cast (by simp)
+:= by
+  refine BitVec.toList_inj ?_
+
+  simp
+  unfold squeeze Spec.sponge.squeeze
+  simp
+  split
+  case isTrue base_case =>
+    simp [base_case, BitVec.toList]
+    ext i
+    · simp [*]
+    simp_lists
+    simp
+    assume i < d
+    case otherwise h => simp [h]
+    simp [*, ‹i < m›']
+    rfl
+  case isFalse _ =>
+    rw [ListIR.sponge.squeeze.refinement]
+    simp [ListIR.list_keccak_p, BitVec.toBitVec_toList]
+    congr
+    simp [BitVec.toList_setWidth]
+termination_by d - m
+decreasing_by scalar_decr_tac
+
+
+-- abbrev List.is_chunks_of(chunks: List (List α))(n: Nat) := ∀ c ∈ chunks, c.length = n
+
+-- @[simp_lists_simps]
+-- theorem List.length_flatten_of_is_chunks(n: Nat)(chunks: List (List α))
+-- : chunks.is_chunks_of n
+-- → chunks.flatten.length = chunks.length * n
+-- := by
+--   intro is_chunks
+
+--   induction chunks
+--   case nil => simp
+--   case cons hd tl ih =>
+--     simp [List.is_chunks_of] at *
+--     obtain ⟨len_hd, len_flatten_tl⟩ := is_chunks
+--     rw [ih (is_chunks := len_flatten_tl)]
+--     simp_arith [*, Nat.add_mul]
+
+-- @[simp_lists_simps]
+-- theorem List.getElem!_cons_div_of_gt[Inhabited α](i n: Nat)(hd: α)(tl: List α)
+-- : n > 0 → i ≥ n → (hd :: tl)[i / n]! = tl[(i - n) / n]!
+-- := by
+--   intro n_pos h
+--   have: i = (i - n) + n := by exact (Nat.sub_eq_iff_eq_add h).mp rfl
+--   conv => lhs; rw [this, Nat.add_div_right (H := n_pos)]
+--   simp
+
+-- @[simp_lists_simps]
+-- theorem List.getElem!_cons_div_of_lt[Inhabited α](i n: Nat)(hd: α)(tl: List α)
+-- : i < n → (hd :: tl)[i / n]! = hd
+-- := by intro h; simp [Nat.div_eq_of_lt, h]
+
+-- @[simp_lists_simps]
+-- theorem List.getElem!_flatten_of_is_chunks(n: Nat)[Inhabited α](chunks: List (List α))
+-- : chunks.is_chunks_of n
+-- → ∀ i, chunks.flatten[i]! = (chunks[i/n]!)[i%n]!
+-- := by
+--   intro is_chunks
+
+--   assume n_pos: n > 0
+--   case otherwise =>
+--     simp at n_pos
+--     intro i
+--     rw [getElem!_default, getElem!_default]
+--     · if inside: i / n < chunks.length then
+--         rw [getElem!_pos]
+--         case h => assumption
+--         have := is_chunks (chunks[i / n]) (by simp)
+--         simp [*]
+--       else
+--         rw [getElem!_neg]
+--         case h => assumption
+--         simp [default]
+--     · rw [List.length_flatten_of_is_chunks (n:=n)]
+--       · simp [*]
+--       · assumption
+
+--   induction chunks
+--   case nil => simp [default]
+--   case cons hd tl ih =>
+--     intro i
+--     simp [List.is_chunks_of] at *
+--     obtain ⟨len_hd, len_flatten_tl⟩ := is_chunks
+--     replace ih := ih len_flatten_tl
+--     by_cases i < n
+--     case pos i_hd =>
+--       simp_lists
+--       simp [Nat.div_eq_of_lt, Nat.mod_eq_of_lt,i_hd]
+--     case neg i_tl =>
+--       simp at i_tl
+--       simp_lists
+--       rw [ih]
+--       simp [len_hd, Nat.mod_eq_sub_mod, i_tl]
+
+-- @[simp_lists_simps]
+-- private theorem List.getElem!_iterate[Inhabited α](f: α → α)(a: α)(n i: Nat)
+-- : (List.iterate f a n)[i]! = if i < n then f^[i] a else default
+-- := by
+--   split
+--   case isTrue i_idx  => simp [getElem!_pos, i_idx]
+--   case isFalse i_oob => simp [getElem!_neg, i_oob]
+
+-- -- def List.sumWhileNotGt(ls: List Nat)(top: Nat) := Id.run do
+-- --   let mut sum := 0
+-- --   for x in ls do
+-- --     if sum + x > top then
+-- --       break
+-- --     sum := sum + x
+-- --   return sum
+
+-- -- theorem List.getElem_flatten[Inhabited α](ls: List (List α))(i: Nat)
+-- -- : let n := ls.map (·.length) |>.sumWhileNotGt i
+-- --   ls.flatten[i]! = (ls[n]!)[i - n]!
+-- -- := by sorry
+
+-- def ref.squeeze(s: List Bool)(n: Nat)(k: Nat := 1600)[NeZero k] :=
+--   (List.iterate list_keccak_p (s.setWidth k) n).flatten
+
+-- attribute [-simp] List.mem_iterate in
+-- @[simp, simp_lists_simps]
+-- theorem iterate_list_keccak_p_is_chunks_of_1600(s: List Bool)(n: Nat)
+-- : (List.iterate ref.list_keccak_p (s.setWidth 1600) n).is_chunks_of 1600
+-- := by
+--   induction n generalizing s
+--   case zero => simp [List.is_chunks_of]
+--   case succ d' ih =>
+--     unfold List.is_chunks_of at *
+--     simp
+--     intros chunk chunk_prev
+--     rw [ih (s := ref.list_keccak_p (s.setWidth 1600))]
+--     simp [*]
+
+-- -- private theorem length_squeeze(n: Nat)(s: List Bool)
+-- -- : (ref.squeeze s n 1600).length = n*1600
+-- -- := by
+-- --   unfold ref.squeeze
+-- --   rw [List.length_flatten_of_is_chunks 1600]
+-- --   case a => apply iterate_list_keccak_p_is_chunks_of_1600
+-- --   simp [ref.squeeze]
+
+-- -- private theorem getElem!_squeeze(n: Nat)(s: List Bool)
+-- -- : (ref.squeeze s n 1600)[i]! = (ref.list_keccak_p^[i / 1600] s.setWidth)[i % 1600]!
+-- -- := by
+-- --   simp [ref.squeeze]
+-- --   ref [List.getElem!_flatten_of_is_chunks]
+-- --   sorry
+
+-- attribute [-simp] List.length_flatten in
+-- attribute [simp] length_iterate_keccak_p in
+-- set_option maxHeartbeats 100000000 in
+-- theorem simple.sponge_squeze_loop.spec (r i: Std.Usize)(input: Std.Slice Bool)(s: Aeneas.Std.Array Bool 1600#usize)
+-- : r.val < 1600
+-- → i < input.length
+-- → i.val % r.val = 0
+-- → input.length + r.val < Std.Usize.max
+-- → ∃ output,
+--   sponge_squeeze_loop r input s i = .ok output ∧
+--   output.length = input.length ∧
+--   output.val = input.val.take i.val ++ ref.squeeze s.val ((input.length - i.val) / r)
+--   /- output.val[j]! = input. -/
+--   /- (∀ j < output.length, output.val[j]! = -/
+--   /-   if i.val ≤ j then -/
+--   /-     (ref.list_keccak_p s.val)[j]! -/
+--   /-   else -/
+--   /-     input.val[j]! -/
+-- := by
+--   intros r_lt i_idx i_mod_r no_overflow
+--   unfold sponge_squeeze_loop
+--   let* ⟨ s1, s1_def ⟩ ← Std.Array.to_slice.progress_spec
+--   let* ⟨ nb_added, curr, nb_added_val, curr_len, curr_pt_val ⟩ ← add_to_vec.spec
+--   · simp [*, Std.Array.to_slice]
+--   let* ⟨ i1, i1_post ⟩ ← Std.Usize.add_spec
+--   have: input.length ≤ (input.length / r) * 1600 := by sorry
+--   split
+--   case isTrue last_loop =>
+--     simp [*]
+--     ext j
+--     · have this2: input.length - i ≤ input.length := by exact Nat.sub_le input.length i.val
+--       simp [*, le_of_lt, _root_.trans this2 this]
+--     assume j_idx: j < curr.length
+--     case otherwise => simp_lists
+--     rw [curr_pt_val]
+--     case a => simpa [*] using j_idx
+--     simp_lists
+--     split
+--     case isTrue cond =>
+--       simp_ifs
+--       rw [List.getElem!_flatten_of_is_chunks 1600]
+--       case a => apply iterate_list_keccak_p_is_chunks_of_1600
+--       simp_lists
+--       have: j < (input.length / r) * 1600 := by
+--         scalar_tac
+--       sorry
+--     rw [List.getElem!_flatten_of_is_chunks]
+--     sorry
+--   case isFalse has_more_loops =>
+--     let* ⟨ s2, s2_post ⟩ ← keccak_p.spec'
+--     let* ⟨ res, res_post_1, res_post_2 ⟩ ← spec
+
+--     simp [*]
+
+-- theorem simple.sponge_squeze.spec (r: Std.Usize)(input: Std.Slice Bool)
+-- : ∃ output,
+--   sponge_squeeze_loop r input s i = .ok output ∧
+--   output.length = input.length ∧
+--   output.val = (List.iterate ref.list_keccak_p s.val (input.length / r)).flatten.take (input.length - i.val)
+-- := by
+--   sorry
+
+-- -- @[progress]
+-- theorem simple.sponge.spec (r : Std.Usize) (bs output suffix: Std.Slice Bool)
+-- [NeZero r.val]
+-- /- (r_ne_zero: r.val ≠ 0) -/
+-- : ∃ output,
+--   simple.sponge r bs output suffix = .ok output ∧
+--   output.val = (Spec.sponge (f := Spec.Keccak.P 6 (nᵣ := 24)) (pad := Spec.«pad10*1») r.val (Array.mk <| bs.val ++ suffix.val ) output.length).toArray.toList
+-- := by sorry
